Rewrote Refresh Rule

theories/ARL/Lib/FreshExtras.v
@@ -3,17 +3,84 @@ From stdpp Require Import prelude fin_maps.
 Section refresh_map.
 
 Context
-  `{Infinite K}
-  `{FinMap K M}.
+  `{Infinite K, FinSet K KSet}.
 
-Fixpoint refresh_map' `{Fresh K C, Union C, Singleton K C}
-    (orig : list K) (X : C) : M K :=
+Fixpoint refresh_list'
+    (orig : list K) (X : KSet) : list (K * K) :=
   match orig with
-  | [] => empty
-  | x :: orig => let x' := fresh X in insert x x' (refresh_map' orig ({[ x' ]} ∪ X))
+  | [] => []
+  | x :: orig => let x' := fresh X in (x, x') :: refresh_list' orig ({[ x' ]} ∪ X)
   end.
 
-Definition refresh_map `{Fresh K C, FinSet K C} (orig : list K) (X : C) : M K :=
-  refresh_map' orig (X ∪ list_to_set orig).
+Definition refresh_list (to_rename to_avoid : KSet) : list (K * K) :=
+  refresh_list' (elements to_rename) (to_avoid ∪ to_rename).
+
+Lemma refresh_list_replacements_are_fresh' (orig : list K) (X : KSet) :
+  forall y, y ∈ (map snd (refresh_list' orig X)) -> y ∉ X.
+Proof.
+  revert X; induction orig; [by inversion 1 | ].
+  cbn; intros ? ?; rewrite elem_of_cons; intros [-> | Hy].
+  - by apply is_fresh.
+  - apply IHorig in Hy.
+    by contradict Hy; apply elem_of_union; right.
+Qed.
+
+Lemma refresh_list_replacements_nodup' :
+  forall orig X , NoDup (map snd (refresh_list' orig X)).
+Proof.
+  induction orig; [by constructor |]; cbn.
+  constructor; [| by apply IHorig].
+  intro Hx; apply refresh_list_replacements_are_fresh' in Hx.
+  by contradict Hx; rewrite elem_of_union, elem_of_singleton; left.
+Qed.
+
+Lemma refresh_list_replacements_nodup :
+  forall orig X, NoDup (map snd (refresh_list orig X)).
+Proof.
+  by intros orig X; apply refresh_list_replacements_nodup'.
+Qed.
+
+Lemma refresh_list_fst' :
+  forall orig X, map fst (refresh_list' orig X) = orig.
+Proof.
+  induction orig; [done |]; cbn.
+  by intro X; f_equal; apply IHorig.
+Qed.
+
+Lemma refresh_list_fst :
+  forall orig X, map fst (refresh_list orig X) = elements orig.
+Proof. by intros; apply refresh_list_fst'. Qed.
+
+Lemma refresh_list_nodup :
+  forall orig X, NoDup (map fst (refresh_list orig X) ++ map snd (refresh_list orig X)).
+Proof.
+  intros.
+  apply NoDup_app; split_and!.
+  - by rewrite refresh_list_fst; apply NoDup_elements.
+  - intro x; rewrite refresh_list_fst, elem_of_elements; intros Hx1 Hx2.
+    eapply refresh_list_replacements_are_fresh'; [done |].
+    by rewrite elem_of_union; right.
+  - apply refresh_list_replacements_nodup.
+Qed.
+
+Lemma refresh_list_replacements_orig :
+  forall orig X, list_to_set (map snd (refresh_list orig X)) ## orig.
+Proof.
+  intros.
+  pose proof (Hnodup := refresh_list_nodup orig X).
+  apply NoDup_app in Hnodup as (_ & Hnodup & _).
+  intros x Hrepl Horig.
+  apply (Hnodup x).
+  - by rewrite refresh_list_fst, elem_of_elements.
+  - by apply elem_of_list_to_set in Hrepl.
+Qed.
+
+Lemma refresh_list_replacements_avoid (orig X : KSet) :
+  list_to_set (map snd (refresh_list orig X)) ## X.
+Proof.
+  intro y; rewrite elem_of_list_to_set; intro Hy.
+  apply refresh_list_replacements_are_fresh' in Hy.
+  by contradict Hy; apply elem_of_union; left.
+Qed.
 
 End refresh_map.
