theories/ARL/QARS/RefreshRule.v
@@ -1,73 +1,8 @@
-From stdpp Require Import prelude.
-From Coq Require Import FunctionalExtensionality.
+From stdpp Require Import prelude fin_maps.
+From Coq Require Import FunctionalExtensionality Classical.
 From sets Require Import Ensemble.
+From ARL Require Import FreshExtras.
 From ARL Require Import TransitionSystem RuleBasedTransitionSystem.
-
-Definition find_position `{EqDecision A} (l : list A) (a : A) : option nat :=
-  fst <$> list_find (fun x => x = a) l.
-
-Lemma find_position_Some `{EqDecision A} (l : list A) a n :
-  find_position l a = Some n -> l !! n = Some a.
-Proof.
-  unfold find_position; intro Hpos.
-  destruct list_find as [(_n, _a) |] eqn: Hlist_find_eq; [| by inversion Hlist_find_eq].
-  apply Some_inj in Hpos; subst n.
-  by apply list_find_Some in Hlist_find_eq as (? & -> & _).
-Qed.
-
-Lemma find_position_elem_of `{EqDecision A} (l : list A) a :
-  a ∈ l <-> is_Some (find_position l a).
-Proof.
-  split.
-  - intro Ha.
-    cut (is_Some (list_find (fun x => x = a) l)).
-    {
-      intros [(_a, n) H_a].
-      by exists _a; unfold find_position; rewrite H_a.
-    }
-    by eapply list_find_elem_of.
-  - intros [n Hn].
-    by apply find_position_Some, elem_of_list_lookup_2 in Hn.
-Qed.
-
-Lemma find_position_None `{EqDecision A} (l : list A) a :
-  find_position l a = None <-> a ∉ l.
-Proof.
-  rewrite find_position_elem_of.
-  by apply eq_None_not_Some.
-Qed.
-
-Definition find_positions `{EqDecision A} (l subl : list A) : list nat :=
-  omap (find_position l) subl.
-
-Lemma find_positions_elem_of `{EqDecision A} (l subl : list A) x :
-  subl ⊆ l ->
-  x ∈ subl ->
-  x ∈ l <-> exists i, i ∈ find_positions l subl /\ l !! i = Some x.
-Proof.
-  induction subl; [by inversion 2 |].
-  intros Hincl.
-  inversion 1; subst.
-  - rewrite find_position_elem_of; split.
-    + intros [i Hi]; exists i.
-      split; [| by apply find_position_Some].
-      unfold find_positions; rewrite elem_of_list_omap.
-      by exists a; split; [left |].
-    + intros (i & Hi & Hlookup).
-      apply find_position_elem_of, elem_of_list_lookup.
-      by eexists.
-  - rewrite IHsubl; [| by set_solver | done].
-    apply exist_proper; intro i.
-    unfold find_positions; rewrite !elem_of_list_omap.
-    split; intros [(_x & H_x & Hpos) Hi]; (split; [| done]); exists _x; (split; [| done]).
-    + by right.
-    + apply find_position_Some in Hpos.
-      rewrite Hpos in Hi.
-      by congruence.
-Qed.
-
-Definition multiple_lookups `(l : list A) (positions : list nat) : list A :=
-  omap (fun i => lookup i l) positions.
 
 Section sec_refresh_rule.
 
@@ -94,389 +29,300 @@ Lemma valuationXchange_other v x y z :
 Proof. by intros; unfold valuationXchange; rewrite !decide_False. Qed.
 
 Definition valuationXchange_iter
-  (v : Valuation Name) (to_replace replacement : list Name) : Valuation Name :=
-    foldr (fun (xy : Name * Name) (p : Valuation Name) => valuationXchange p xy.1 xy.2)
-      v (zip to_replace replacement).
+  (v : Valuation Name) (subst : list (Name * Name)) : Valuation Name :=
+    foldr (fun xy (p : Valuation Name) => valuationXchange p xy.1 xy.2) v subst.
 
-Lemma valuationXchange_iter_cons v x xs y ys :
-  valuationXchange_iter v (x :: xs) (y :: ys)
-    =
-  valuationXchange (valuationXchange_iter v xs ys) x y.
-Proof. done. Qed.
-
-Lemma valuationXchange_iter_other v to_replace replacement :
+Lemma valuationXchange_iter_other
+  (subst : list (Name * Name)) (to_replace := map fst subst) (replacement := map snd subst) :
   forall x, x ∉ to_replace -> x ∉ replacement ->
-  valuationXchange_iter v to_replace replacement x = v x.
+  forall v, valuationXchange_iter v subst x = v x.
 Proof.
-  revert v replacement; induction to_replace; [done |].
-  intros v replacement x Hx1 Hx2.
-  apply not_elem_of_cons in Hx1 as [Hxa Hx1].
-  destruct replacement as [| r replacement]; [done |].
-  apply not_elem_of_cons in Hx2 as [Hxr Hx2].
-  rewrite valuationXchange_iter_cons, valuationXchange_other by done.
-  by apply IHto_replace.
+  unfold valuationXchange_iter; induction subst; [done |].
+  subst to_replace replacement; cbn.
+  intro x; rewrite !not_elem_of_cons; intros [Hna1 Hnx1] [Hna2 Hnx2] v.
+  unfold valuationXchange at 1.
+  rewrite !decide_False by done.
+  by apply IHsubst.
 Qed.
 
-Lemma valuationXchange_iter_replaced v to_replace replacement :
-  NoDup to_replace ->
-  NoDup replacement ->
-  (forall x, x ∈ to_replace -> x ∈ replacement -> False) ->
-  forall n,
-  forall x, to_replace !! n = Some x ->
-  forall y, replacement !! n = Some y ->
-  valuationXchange_iter v to_replace replacement x = v y
-    /\
-  valuationXchange_iter v to_replace replacement y = v x.
+Lemma valuationXchange_iter_replaced
+  (subst : list (Name * Name)) (to_replace := map fst subst) (replacement := map snd subst) :
+  NoDup (to_replace ++ replacement) ->
+  forall xy, xy ∈ subst ->
+  forall v, valuationXchange_iter v subst xy.1 = v xy.2 /\ valuationXchange_iter v subst xy.2 = v xy.1.
 Proof.
-  revert replacement; induction to_replace; [done |].
-  intros replacement Hnodup1 Hnodup2 Hdisj n x Hx y Hy.
-  destruct replacement as [| b]; [by inversion Hy |].
-  rewrite valuationXchange_iter_cons.
-  apply NoDup_cons in Hnodup1 as [Ha Hnodup1].
-  apply NoDup_cons in Hnodup2 as [Hb Hnodup2].
-  destruct n.
-  - inversion Hx; inversion Hy; subst; clear Hx Hy.
-    rewrite valuationXchange_left, valuationXchange_right.
-    split; apply valuationXchange_iter_other; [| done | done |].
-    + by intro Hy; eapply Hdisj; [right | left].
-    + by intro Hx; eapply Hdisj; [left | right].
-  - cbn in Hx, Hy.
-    rewrite !valuationXchange_other; cycle 1.
-    + intros ->; eapply Hdisj; [by left |]; right.
-      by apply elem_of_list_lookup; eexists.
-    + by contradict Hb; subst; apply elem_of_list_lookup; eexists.
-    + by contradict Ha; subst; apply elem_of_list_lookup; eexists.
-    + intros ->; eapply Hdisj; [| by left]; right.
-      by apply elem_of_list_lookup; eexists.
-    + eapply IHto_replace; [done | done | | done..].
-      by intros; eapply Hdisj; right.
+  induction subst; [by inversion 2 |].
+  rewrite NoDup_app; subst to_replace replacement; cbn.
+  rewrite !NoDup_cons; intros ([Hna1 Hnodup1] & Hdisj' & Hna2 & Hnodup2) xy.
+  assert (Hna1' : a.1 ∉ map snd subst)
+    by (intros Ha1; apply (Hdisj' a.1); [left | right]; done).
+  assert (Hna2' : a.2 ∉ map fst subst)
+    by (intros Ha2; apply (Hdisj' a.2); [right | left]; done).
+  assert (Hna12 : a.1 <> a.2)
+    by (intros Heq; rewrite Heq in Hdisj'; apply (Hdisj' a.2); left).
+  assert (Hdisj : forall x, x ∈ map fst subst -> x ∉ map snd subst)
+    by (intros x Hx1 Hx2; apply (Hdisj' x); right; done).
+  rewrite elem_of_cons; intros [-> | Hxy].
+  - split; unfold valuationXchange at 1.
+    + rewrite decide_True by done.
+      by apply valuationXchange_iter_other.
+    + rewrite decide_False, decide_True by done.
+      by apply valuationXchange_iter_other.
+  - rewrite elem_of_list_fmap in Hna1, Hna2, Hna1', Hna2'.
+    intro v; rewrite !valuationXchange_other.
+    + by apply IHsubst; [apply NoDup_app |].
+    + by contradict Hna1'; eexists.
+    + by contradict Hna2; eexists.
+    + by contradict Hna1; eexists.
+    + by contradict Hna2'; eexists.
 Qed.
 
-Lemma valuationXchange_iter_left v to_replace replacement :
-  NoDup to_replace ->
-  NoDup replacement ->
-  (forall x, x ∈ to_replace -> x ∈ replacement -> False) ->
-  forall n,
-  forall x, to_replace !! n = Some x ->
-  forall y, replacement !! n = Some y ->
-  valuationXchange_iter v to_replace replacement x = v y.
-Proof.
-  by intros; eapply valuationXchange_iter_replaced with (x := x).
-Qed.
+Lemma valuationXchange_iter_left
+  (subst : list (Name * Name)) (to_replace := map fst subst) (replacement := map snd subst) :
+  NoDup (to_replace ++ replacement) ->
+  forall xy, xy ∈ subst ->
+  forall v, valuationXchange_iter v subst xy.1 = v xy.2.
+Proof. by intros; apply valuationXchange_iter_replaced. Qed.
 
-Lemma valuationXchange_iter_right v to_replace replacement :
-  NoDup to_replace ->
-  NoDup replacement ->
-  (forall x, x ∈ to_replace -> x ∈ replacement -> False) ->
-  forall n,
-  forall x, to_replace !! n = Some x ->
-  forall y, replacement !! n = Some y ->
-  valuationXchange_iter v to_replace replacement y = v x.
-Proof.
-  by intros; eapply valuationXchange_iter_replaced with (x := x).
-Qed.
+Lemma valuationXchange_iter_right
+  (subst : list (Name * Name)) (to_replace := map fst subst) (replacement := map snd subst) :
+  NoDup (to_replace ++ replacement) ->
+  forall xy, xy ∈ subst ->
+  forall v, valuationXchange_iter v subst xy.2 = v xy.1.
+Proof. by intros; apply valuationXchange_iter_replaced. Qed.
 
-Lemma valuationXchange_iter_twice v to_replace replacement :
-  NoDup to_replace ->
-  NoDup replacement ->
-  (forall x, x ∈ to_replace -> x ∈ replacement -> False) ->
-  length to_replace = length replacement ->
-  valuationXchange_iter (valuationXchange_iter v to_replace replacement)
-    to_replace replacement = v.
+Lemma valuationXchange_iter_twice
+  (subst : list (Name * Name)) (to_replace := map fst subst) (replacement := map snd subst) :
+  NoDup (to_replace ++ replacement) ->
+  forall v, valuationXchange_iter (valuationXchange_iter v subst) subst = v.
 Proof.
-  intros Hnodup1 Hnodup2 Hdisj Hlength.
+  intros Hnodup v.
   extensionality x.
-  destruct (decide (x ∈ to_replace)) as [Hx | Hnx];
-    [| destruct (decide (x ∈ replacement)) as [Hx' | Hnx']].
-  - apply elem_of_list_lookup in Hx as [n Hx].
-    apply lookup_lt_Some in Hx as Hn.
-    rewrite Hlength in Hn.
-    apply lookup_lt_is_Some in Hn as [y Hy].
-    rewrite valuationXchange_iter_left with (n := n) (y := y) by done.
-    by rewrite valuationXchange_iter_right with (n := n) (x := x).
-  - apply elem_of_list_lookup in Hx' as [n Hx'].
-    apply lookup_lt_Some in Hx' as Hn.
-    rewrite <- Hlength in Hn.
-    apply lookup_lt_is_Some in Hn as [y Hy].
-    rewrite valuationXchange_iter_right with (n := n) (x := y) by done.
-    by rewrite valuationXchange_iter_left with (n := n) (y := x).
-  - by rewrite !valuationXchange_iter_other.
+  destruct (decide (x ∈ to_replace ++ replacement)) as [Hin | Hnin];
+    [apply elem_of_app in Hin as [Hin | Hin] |].
+  - apply elem_of_list_fmap in Hin as (xy & -> & Hxy).
+    by rewrite valuationXchange_iter_left, valuationXchange_iter_right.
+  - apply elem_of_list_fmap in Hin as (xy & -> & Hxy).
+    by rewrite valuationXchange_iter_right, valuationXchange_iter_left.
+  - apply not_elem_of_app in Hnin as [].
+    by etransitivity; apply valuationXchange_iter_other.
 Qed.
 
 Definition qpattern_rename_vars_with
-  (p : quantified_pattern) (to_rename renaming : list Name)
-  : quantified_pattern :=
-  fun v => p (valuationXchange_iter v to_rename renaming).
+  (p : quantified_pattern) (subst : list (Name * Name)) : quantified_pattern :=
+  fun v => p (valuationXchange_iter v subst).
 
 Definition qterm_rename_vars_with
-  (p : quantified_term) (to_rename renaming : list Name)
-  : quantified_term :=
-  fun v => p (valuationXchange_iter v to_rename renaming).
+  (p : quantified_term) (subst : list (Name * Name)) : quantified_term :=
+  fun v => p (valuationXchange_iter v subst).
 
-Lemma qterm_rename_vars_with_valuation p to_rename renaming v :
-  qterm_rename_vars_with p to_rename renaming v
+Lemma qterm_rename_vars_with_valuation p subst v :
+  qterm_rename_vars_with p subst v
     =
-  p (valuationXchange_iter v to_rename renaming).
+  p (valuationXchange_iter v subst).
 Proof. done. Qed.
 
-Lemma arl_vars_eq_rename_iter vars1 vars2_list v1 v2 :
-  length vars2_list = size vars1 ->
-  NoDup vars2_list ->
-  vars1 ## list_to_set vars2_list ->
-  ARLVarsEq NameSet (list_to_set vars2_list) v1 v2 ->
-  ARLVarsEq NameSet vars1
-    (valuationXchange_iter v1 (elements vars1) vars2_list)
-    (valuationXchange_iter v2 (elements vars1) vars2_list).
+Existing Instance elem_of_dec_slow.
+
+Lemma arl_vars_eq_rename_iter_sub subst v1 v2
+  (to_replace := map fst subst) (replacement := map snd subst)
+  (to_replace_set : NameSet := list_to_set to_replace)
+  (replacement_set : NameSet := list_to_set replacement) :
+  NoDup (to_replace ++ replacement) ->
+  forall (vars_to_replace : NameSet)
+    (vars_replacement := list_to_set (map snd (filter (fun xy => xy.1 ∈ vars_to_replace) subst))),
+    vars_to_replace ⊆ to_replace_set ->
+  ARLVarsEq NameSet vars_replacement v1 v2 ->
+  ARLVarsEq NameSet vars_to_replace
+    (valuationXchange_iter v1 subst)
+    (valuationXchange_iter v2 subst).
 Proof.
-  intros Hlen Hnodup2 Hdisj Heqvars.
+  intros Hnodup ? ? Hincl Heq.
   constructor; intros x Hx.
-  apply elem_of_elements in Hx as Hex.
-  apply elem_of_list_lookup in Hex as [n Hnx].
-  apply lookup_lt_Some in Hnx as Hn.
-  unfold size, set_size in Hlen; cbn in Hlen.
-  rewrite <- Hlen in Hn.
-  apply lookup_lt_is_Some in Hn as [y Hny].
-  rewrite !valuationXchange_iter_left with (n := n) (y := y).
-  - by apply Heqvars, elem_of_list_to_set, elem_of_list_lookup; eexists.
-  - by apply NoDup_elements.
-  - done.
-  - by intros; eapply Hdisj; [apply elem_of_elements | apply elem_of_list_to_set].
-  - done.
-  - done.
-  - by apply NoDup_elements.
-  - done.
-  - by intros; eapply Hdisj; [apply elem_of_elements | apply elem_of_list_to_set].
-  - done.
-  - done.
+  apply Hincl in Hx as Hx'.
+  apply elem_of_list_to_set, elem_of_list_fmap in Hx' as (xy & -> & Hxy).
+  rewrite !valuationXchange_iter_left by done.
+  apply Heq, elem_of_list_to_set, elem_of_list_fmap.
+  by eexists; rewrite elem_of_list_filter.
 Qed.
 
-Lemma pattern_dependent_vars_rename_pattern p vars1 vars2_list :
+Lemma arl_vars_eq_rename_iter subst v1 v2
+  (to_replace := map fst subst) (replacement := map snd subst)
+  (to_replace_set : NameSet := list_to_set to_replace)
+  (replacement_set : NameSet := list_to_set replacement) :
+  NoDup (to_replace ++ replacement) ->
+  ARLVarsEq NameSet replacement_set v1 v2 ->
+  ARLVarsEq NameSet to_replace_set
+    (valuationXchange_iter v1 subst)
+    (valuationXchange_iter v2 subst).
+Proof.
+  intros Hnodup Heq.
+  constructor; intros x Hx.
+  apply elem_of_list_to_set, elem_of_list_fmap in Hx as (xy & -> & Hxy).
+  rewrite !valuationXchange_iter_left by done.
+  apply Heq, elem_of_list_to_set, elem_of_list_fmap.
+  by eexists.
+Qed.
+
+Lemma pattern_dependent_vars_rename_pattern_sub p vars1 subst
+  (to_replace := map fst subst) (replacement := map snd subst) :
+  NoDup (to_replace ++ replacement) ->
   pattern_dependent_vars NameSet p vars1 ->
-  length vars2_list = size vars1 ->
-  NoDup vars2_list ->
-  vars1 ## list_to_set vars2_list ->
-  pattern_dependent_vars NameSet (qpattern_rename_vars_with p (elements vars1) vars2_list) (list_to_set vars2_list).
+  vars1 ⊆ list_to_set to_replace ->
+  let vars2 := list_to_set (map snd (filter (fun xy => xy.1 ∈ vars1) subst)) in
+  pattern_dependent_vars NameSet (qpattern_rename_vars_with p subst) vars2.
 Proof.
-  intros Hfve Hlen Hnodup2 Hdisj v1 v2 Heqvars.
-  by apply Hfve, arl_vars_eq_rename_iter.
+  intros Hnodup Hdep Hinc vars2 v1 v2 Heq.
+  by apply Hdep, arl_vars_eq_rename_iter_sub.
 Qed.
 
-Lemma pattern_dependent_vars_rename_term (p : quantified_term) vars1 vars2_list :
+Lemma pattern_dependent_vars_rename_pattern p subst
+  (to_replace := map fst subst) (replacement := map snd subst) :
+  NoDup (to_replace ++ replacement) ->
+  pattern_dependent_vars NameSet p (list_to_set to_replace) ->
+  pattern_dependent_vars NameSet (qpattern_rename_vars_with p subst) (list_to_set replacement).
+Proof.
+  intros Hnodup Hdep v1 v2 Heq.
+  by apply Hdep, arl_vars_eq_rename_iter.
+Qed.
+
+Lemma pattern_dependent_vars_rename_term_sub (p : quantified_term) vars1 subst
+  (to_replace := map fst subst) (replacement := map snd subst) :
+  NoDup (to_replace ++ replacement) ->
   pattern_dependent_vars NameSet p vars1 ->
-  length vars2_list = size vars1 ->
-  NoDup vars2_list ->
-  vars1 ## list_to_set vars2_list ->
-  pattern_dependent_vars NameSet (qterm_rename_vars_with p (elements vars1) vars2_list) (list_to_set vars2_list).
+  vars1 ⊆ list_to_set to_replace ->
+  let vars2 := list_to_set (map snd (filter (fun xy => xy.1 ∈ vars1) subst)) in
+  pattern_dependent_vars NameSet (qterm_rename_vars_with p subst) vars2.
 Proof.
-  intros Hfve Hlen Hnodup2 Hdisj v1 v2 Heqvars.
-  by apply Hfve, arl_vars_eq_rename_iter.
+  intros Hnodup Hdep Hinc vars2 v1 v2 Heq.
+  by apply Hdep, arl_vars_eq_rename_iter_sub.
 Qed.
 
-Lemma qterm_rename_vars_with_valuation_rev (p : quantified_term) to_rename renaming :
-  pattern_dependent_vars NameSet p (list_to_set to_rename) ->
-  NoDup to_rename ->
-  NoDup renaming ->
-  length to_rename = length renaming ->
-  (forall x, x ∈ to_rename -> x ∈ renaming -> False) ->
-  forall v, p v = qterm_rename_vars_with p to_rename renaming (valuationXchange_iter v to_rename renaming).
+Lemma pattern_dependent_vars_rename_term (p : quantified_term) subst
+  (to_replace := map fst subst) (replacement := map snd subst) :
+  NoDup (to_replace ++ replacement) ->
+  pattern_dependent_vars NameSet p (list_to_set to_replace) ->
+  pattern_dependent_vars NameSet (qterm_rename_vars_with p subst) (list_to_set replacement).
 Proof.
-  intros Henough Hnodup1 Hnodup2 Hlength Hdisj v; unfold qterm_rename_vars_with.
-  apply (Henough v (valuationXchange_iter (valuationXchange_iter v to_rename renaming)
-    to_rename renaming)); [| done].
-  constructor; intros x Hx.
-  by rewrite valuationXchange_iter_twice.
+  intros Hnodup Hdep v1 v2 Heq.
+  by apply Hdep, arl_vars_eq_rename_iter.
 Qed.
 
-Lemma qpattern_rename_vars_with_valuation_rev p to_rename renaming :
-  pattern_dependent_vars NameSet p (list_to_set to_rename) ->
-  NoDup to_rename ->
-  NoDup renaming ->
-  length to_rename = length renaming ->
-  (forall x, x ∈ to_rename -> x ∈ renaming -> False) ->
-  forall v, p v ≡ qpattern_rename_vars_with p to_rename renaming (valuationXchange_iter v to_rename renaming).
+Lemma qterm_rename_vars_with_valuation_rev (p : quantified_term) subst
+  (to_replace := map fst subst) (replacement := map snd subst) :
+  NoDup (to_replace ++ replacement) ->
+  forall v, p v = qterm_rename_vars_with p subst (valuationXchange_iter v subst).
 Proof.
-  intros Henough Hnodup1 Hnodup2 Hlength Hdisj v; unfold qterm_rename_vars_with.
-  apply (Henough v (valuationXchange_iter (valuationXchange_iter v to_rename renaming)
-    to_rename renaming)).
-  constructor; intros x Hx.
-  by rewrite valuationXchange_iter_twice.
+  unfold qterm_rename_vars_with.
+  by intros; rewrite valuationXchange_iter_twice.
 Qed.
 
-Context `{Infinite Name}.
+Lemma qpattern_rename_vars_with_valuation_rev p subst
+  (to_replace := map fst subst) (replacement := map snd subst) :
+  NoDup (to_replace ++ replacement) ->
+  forall v, p v = qpattern_rename_vars_with p subst (valuationXchange_iter v subst).
+Proof.
+  unfold qpattern_rename_vars_with.
+  by intros; rewrite valuationXchange_iter_twice.
+Qed.
+
+Context
+  `{Infinite Name}.
 
 Program Definition rewrite_rule_refresh_vars (r : RewriteRule NameSet) (avoid : NameSet) : RewriteRule NameSet :=
-  let vars_list := elements (vars r) in
-  let fresh_vars := fresh_list (length vars_list) (avoid ∪ vars r) in
-  let vars_lhs_positions := find_positions vars_list (elements (vars_lhs r)) in
-  let fresh_vars_lhs := multiple_lookups fresh_vars vars_lhs_positions in
+  let subst := refresh_list (vars r) avoid in
+  let subst_lhs := filter (fun xy => xy.1 ∈ vars_lhs r) subst in
   {|
-    vars := list_to_set fresh_vars;
-    vars_lhs := list_to_set fresh_vars_lhs;
-    lhs := qterm_rename_vars_with (lhs r) vars_list fresh_vars;
-    requires := qpattern_rename_vars_with (requires r) vars_list fresh_vars;
-    rhs := qterm_rename_vars_with (rhs r) vars_list fresh_vars;
-    ensures := qpattern_rename_vars_with (ensures r) vars_list fresh_vars;
+    vars := list_to_set (map snd subst) ;
+    vars_lhs := list_to_set (map snd subst_lhs) ;
+    lhs := qterm_rename_vars_with (lhs r) subst ;
+    requires := qpattern_rename_vars_with (requires r) subst ;
+    rhs := qterm_rename_vars_with (rhs r) subst ;
+    ensures := qpattern_rename_vars_with (ensures r) subst ;
   |}.
 Next Obligation.
-  intros * x.
-  rewrite !elem_of_list_to_set; intro Hx.
-  apply elem_of_list_omap in Hx as (? & ? & ?).
-  by apply elem_of_list_lookup; eexists.
-Qed.
-Next Obligation.
-  intros * v1 v2 Heqvars.
-  apply lhs_vars.
-  specialize (arl_vars_eq_rename_iter (vars_lhs r) fresh_vars_lhs v1 v2).
-Next Obligation.
-  intros [] * ?; apply ensures_predicate.
+  cbn; intros r avoid y; rewrite !elem_of_list_to_set, !elem_of_list_fmap.
+  intros (xy & -> & Hxy).
+  apply elem_of_list_filter in Hxy as [].
+  by eexists.
 Qed.
 Next Obligation.
   intros.
-  eapply pattern_dependent_vars_rename_term.
-  - by apply lhs_vars.
-  - by apply fresh_list_length.
-  - apply NoDup_fresh_list.
-  - intros x Hx1 Hx2.
-    eapply Forall_fresh_elem_of.
-    + apply Forall_fresh_list.
-    + by apply elem_of_list_to_set in Hx2.
-    + by apply elem_of_union; right.
+  apply pattern_dependent_vars_rename_term_sub;
+    [by apply refresh_list_nodup | by apply lhs_vars |].
+  subst subst; rewrite refresh_list_fst, list_to_set_elements.
+  by apply vars_lhs_prop.
 Qed.
 Next Obligation.
   intros.
-  eapply pattern_dependent_vars_rename_term.
-  - by apply rhs_vars.
-  - by apply fresh_list_length.
-  - apply NoDup_fresh_list.
-  - intros x Hx1 Hx2.
-    eapply Forall_fresh_elem_of.
-    + apply Forall_fresh_list.
-    + by apply elem_of_list_to_set in Hx2.
-    + by apply elem_of_union; right.
+  apply pattern_dependent_vars_rename_term;
+    [by apply refresh_list_nodup |].
+  subst subst; rewrite refresh_list_fst, list_to_set_elements.
+  by apply rhs_vars.
 Qed.
 Next Obligation.
   intros.
-  eapply pattern_dependent_vars_rename_pattern.
-  - by apply requires_vars.
-  - by apply fresh_list_length.
-  - apply NoDup_fresh_list.
-  - intros x Hx1 Hx2.
-    eapply Forall_fresh_elem_of.
-    + apply Forall_fresh_list.
-    + by apply elem_of_list_to_set in Hx2.
-    + by apply elem_of_union; right.
+  apply pattern_dependent_vars_rename_pattern_sub;
+    [by apply refresh_list_nodup | by apply requires_vars |].
+  subst subst; rewrite refresh_list_fst, list_to_set_elements.
+  by apply vars_lhs_prop.
 Qed.
 Next Obligation.
   intros.
-  eapply pattern_dependent_vars_rename_pattern.
-  - by apply ensures_vars.
-  - by apply fresh_list_length.
-  - apply NoDup_fresh_list.
-  - intros x Hx1 Hx2.
-    eapply Forall_fresh_elem_of.
-    + apply Forall_fresh_list.
-    + by apply elem_of_list_to_set in Hx2.
-    + by apply elem_of_union; right.
+  apply pattern_dependent_vars_rename_pattern;
+    [by apply refresh_list_nodup |].
+  subst subst; rewrite refresh_list_fst, list_to_set_elements.
+  by apply ensures_vars.
+Qed.
+Next Obligation.
+  by intros; intro; apply requires_predicate.
+Qed.
+Next Obligation.
+  by intros; intro; apply ensures_predicate.
 Qed.
 
 Lemma rewrite_rule_refresh_vars_disj r avoid :
   vars (rewrite_rule_refresh_vars r avoid) ## (avoid ∪ vars r).
 Proof.
-  cbn; intros x Hx1 Hx2.
-  eapply Forall_fresh_elem_of.
-  + apply Forall_fresh_list.
-  + by apply elem_of_list_to_set in Hx1.
-  + done.
+  cbn; intro x; rewrite elem_of_union; intros ? [].
+  - by eapply @refresh_list_replacements_avoid with (KSet := NameSet).
+  - by eapply @refresh_list_replacements_orig with (KSet := NameSet).
 Qed.
 
 Lemma rewrite_rule_refresh_vars_disj_original r avoid :
   vars (rewrite_rule_refresh_vars r avoid) ## vars r.
-Proof.
-  cbn; intros x Hx1 Hx2.
-  eapply rewrite_rule_refresh_vars_disj; [by exact Hx1 |].
-  by apply elem_of_union; right.
-Qed.
+Proof. by apply refresh_list_replacements_orig. Qed.
 
 Lemma rewrite_rule_refresh_vars_disj_avoid r avoid :
   vars (rewrite_rule_refresh_vars r avoid) ## avoid.
-Proof.
-  cbn; intros x Hx1 Hx2.
-  eapply rewrite_rule_refresh_vars_disj; [by exact Hx1 |].
-  by apply elem_of_union; left.
-Qed.
+Proof. by apply refresh_list_replacements_avoid. Qed.
 
 #[local] Lemma TransitionFromRuleInstance_refresh_vars r avoid
   (refreshed := rewrite_rule_refresh_vars r avoid)
-  (vars_list := elements (vars r))
-  (fresh_vars := fresh_list (length vars_list) (avoid ∪ vars r))
+  (subst := refresh_list (vars r) avoid)
   (v : Valuation Name)
   (a b : idomain) :
   TransitionFromRuleInstance r v a b
     ->
-  TransitionFromRuleInstance
-    (rewrite_rule_refresh_vars r avoid)
-    (valuationXchange_iter v vars_list fresh_vars)
-    a b.
+  TransitionFromRuleInstance refreshed (valuationXchange_iter v subst) a b.
 Proof.
+  pose proof (Hnodup := refresh_list_nodup (vars r) avoid).
   intros []; constructor; cbn.
-  - unfold qterm_rename_vars_with.
-    rewrite valuationXchange_iter_twice.
-    + done.
-    + apply NoDup_elements.
-    + apply NoDup_fresh_list.
-    + intros x Hx1 Hx2.
-      eapply Forall_fresh_elem_of.
-      * apply Forall_fresh_list.
-      * done.
-      * by apply elem_of_union; right; apply elem_of_elements.
-    + by rewrite fresh_list_length.
-  - unfold qterm_rename_vars_with.
-    rewrite valuationXchange_iter_twice.
-    + done.
-    + apply NoDup_elements.
-    + apply NoDup_fresh_list.
-    + intros x Hx1 Hx2.
-      eapply Forall_fresh_elem_of.
-      * apply Forall_fresh_list.
-      * done.
-      * by apply elem_of_union; right; apply elem_of_elements.
-    + by rewrite fresh_list_length.
-  - unfold qpattern_rename_vars_with.
-    rewrite valuationXchange_iter_twice.
-    + done.
-    + apply NoDup_elements.
-    + apply NoDup_fresh_list.
-    + intros x Hx1 Hx2.
-      eapply Forall_fresh_elem_of.
-      * apply Forall_fresh_list.
-      * done.
-      * by apply elem_of_union; right; apply elem_of_elements.
-    + by rewrite fresh_list_length.
-  - unfold qpattern_rename_vars_with.
-    rewrite valuationXchange_iter_twice.
-    + done.
-    + apply NoDup_elements.
-    + apply NoDup_fresh_list.
-    + intros x Hx1 Hx2.
-      eapply Forall_fresh_elem_of.
-      * apply Forall_fresh_list.
-      * done.
-      * by apply elem_of_union; right; apply elem_of_elements.
-    + by rewrite fresh_list_length.
+  - by rewrite <- qterm_rename_vars_with_valuation_rev.
+  - by rewrite <- qterm_rename_vars_with_valuation_rev.
+  - by rewrite <- qpattern_rename_vars_with_valuation_rev.
+  - by rewrite <- qpattern_rename_vars_with_valuation_rev.
 Qed.
 
 #[local] Lemma TransitionFromRuleInstance_refresh_vars_rev r avoid
   (refreshed := rewrite_rule_refresh_vars r avoid)
-  (vars_list := elements (vars r))
-  (fresh_vars := fresh_list (length vars_list) (avoid ∪ vars r))
+  (subst := refresh_list (vars r) avoid)
   (v : Valuation Name)
   (a b : idomain) :
-  TransitionFromRuleInstance
-    (rewrite_rule_refresh_vars r avoid) v a b
+  TransitionFromRuleInstance refreshed v a b
     ->
-  TransitionFromRuleInstance
-    r (valuationXchange_iter v vars_list fresh_vars) a b.
-Proof. by intros []; constructor; cbn; done. Qed.
+  TransitionFromRuleInstance r (valuationXchange_iter v subst) a b.
+Proof. by intros []; constructor. Qed.
 
 Lemma TransitionFromRule_refresh_vars r avoid :
   forall a b, TransitionFromRule r a b <->
